src/Iris/Std.lean
@@ -1,6 +1,5 @@
 import Iris.Std.Classes
 import Iris.Std.Expr
-import Iris.Std.List
 import Iris.Std.Prod
 import Iris.Std.Rewrite
 import Iris.Std.Tactic
