src/Iris/Std/Prod.lean
@@ -1,12 +1,5 @@
 namespace Prod
 
-def allSome? : Option α × Option β → Option (α × β)
-  | (some x, some y) => some (x, y)
-  | _                => none
-
-def mapAll (f : α → β) : α × α → β × β
-  | (x, y) => (f x, f y)
-
 def mapAllM [Monad M] (f : α → M β) : α × α → M (β × β)
   | (x, y) => do return (← f x, ← f y)
 
